stash

isabelle/CoreVerse.thy
@@ -35,65 +35,8 @@ nominal_datatype "exp" =
 | Var var
 | Const int
 | Unit
-| Tuple exp exp
+| Tup exp exp
 | Lam x::var e::exp binds x in e
-
-
-subsection \<open>Ad-hoc methods for nominal-functions over lambda terms\<close>
-
-ML \<open>
-fun graph_aux_tac ctxt =
-  SUBGOAL (fn (subgoal, i) =>
-    (case subgoal of
-      Const (@{const_name Trueprop}, _) $ (Const (@{const_name eqvt}, _) $ Free (f, _)) =>
-        full_simp_tac (
-          ctxt addsimps [@{thm eqvt_def}, Proof_Context.get_thm ctxt (f ^ "_def")]) i
-    | _ => no_tac))
-\<close>
-
-method_setup eqvt_graph_aux =
-  \<open>Scan.succeed (fn ctxt : Proof.context => SIMPLE_METHOD' (graph_aux_tac ctxt))\<close>
-  "show equivariance of auxilliary graph construction for nominal functions"
-
-method without_alpha_lst methods m =
-  (match termI in H [simproc del: alpha_lst]: _ \<Rightarrow> \<open>m\<close>)
-
-method Abs_lst =
-  (match premises in
-    "atom ?x \<sharp> c" and P [thin]: "[[atom _]]lst. _ = [[atom _]]lst. _" for c :: "'a::fs" \<Rightarrow>
-      \<open>rule Abs_lst1_fcb2' [where c = c, OF P]\<close>
-  \<bar> P [thin]: "[[atom _]]lst. _ = [[atom _]]lst. _" \<Rightarrow> \<open>rule Abs_lst1_fcb2' [where c = "()", OF P]\<close>)
-
-find_theorems name:strong_exhaust
-
-method pat_comp_aux =
-  (match premises in
-    "x = (_ :: exp) \<Longrightarrow> _" for x \<Rightarrow> \<open>rule exp.strong_exhaust [where y = x and c = x]\<close>
-  \<bar> "x = (Var _, _) \<Longrightarrow> _" for x :: "_ :: fs" \<Rightarrow>
-    \<open>rule exp.strong_exhaust [where y = "fst x" and c = x]\<close>
-  \<bar> "x = (_, Var _) \<Longrightarrow> _" for x :: "_ :: fs" \<Rightarrow>
-    \<open>rule exp.strong_exhaust [where y = "snd x" and c = x]\<close>
-  \<bar> "x = (_, _, Var _) \<Longrightarrow> _" for x :: "_ :: fs" \<Rightarrow>
-    \<open>rule exp.strong_exhaust [where y = "snd (snd x)" and c = x]\<close>
-)
-
-method pat_comp = (pat_comp_aux; force simp: fresh_star_def fresh_Pair_elim)
-
-method freshness uses fresh =
-  (match conclusion in
-    "_ \<sharp> _" \<Rightarrow> \<open>simp add: fresh_Unit fresh_Pair fresh\<close>
-  \<bar> "_ \<sharp>* _" \<Rightarrow> \<open>simp add: fresh_star_def fresh_Unit fresh_Pair fresh\<close>)
-
-method solve_eqvt_at =
-  (simp add: eqvt_at_def; simp add: perm_supp_eq fresh_star_Pair)+
-
-method nf uses fresh = without_alpha_lst \<open>
-  eqvt_graph_aux, rule TrueI, pat_comp, auto, Abs_lst,
-  auto simp: Abs_fresh_iff pure_fresh perm_supp_eq,
-  (freshness fresh: fresh)+,
-  solve_eqvt_at?\<close>
-
-
 
 subsection \<open>Substitutions\<close>
 
@@ -106,16 +49,204 @@ where
 | "atom y \<sharp> (x, s) \<Longrightarrow> subst x s (Def y e) = Def y (subst x s e)"
 | "subst x s (App t u) = App (subst x s t) (subst x s u)"
 | "subst x s (Var y) = (if x = y then s else Var y)"
+| "subst x s (Const k) = Const k"
+| "subst x s Unit = Unit"
+| "subst x s (Tup v1 v2) = Tup (subst x s v1) (subst x s v2)"
 | "atom y \<sharp> (x, s) \<Longrightarrow> subst x s (Lam y t) = Lam y (subst x s t)"
 proof goal_cases
   case (3 P x)
-  show ?case  sorry
+  then show ?case 
+  proof (cases x)
+    case (fields a b c)
+    then show ?thesis using 3
+      by (rule_tac exp.strong_exhaust[of c _ "(a,b)"])
+         (auto simp add: fresh_star_def)
+  qed
 next
-  apply_end (auto simp add: eqvt_def subst_graph_def) 
-
+  case (42 y x s e y' x' s' e')
+  then show ?case sorry
+next
+  case (69 y x s t y' x' s' t')
+  then show ?case sorry
 qed (auto simp add: eqvt_def subst_graph_aux_def)
 
 nominal_termination (eqvt) by lexicographic_order
+
+
+inductive is_exp :: "exp \<Rightarrow> bool" and is_val :: "exp \<Rightarrow> bool" where
+  is_exp_Val: "is_val e \<Longrightarrow> is_exp e"
+| is_exp_Seq: "is_exp e1 \<Longrightarrow> is_exp e2 \<Longrightarrow> is_exp (Seq e1 e2)"
+| is_exp_Bar: "is_exp e1 \<Longrightarrow> is_exp e2 \<Longrightarrow> is_exp (Bar e1 e2)"
+| is_exp_App: "is_val e1 \<Longrightarrow> is_val e2 \<Longrightarrow> is_exp (App e1 e2)"
+| is_exp_Def: "is_exp e \<Longrightarrow> is_exp (Def x e)"
+| is_exp_One: "is_exp e \<Longrightarrow> is_exp (One e)"
+| is_exp_All: "is_exp e \<Longrightarrow> is_exp (All e)"
+(* Now the values *)
+| is_val_Var: "is_val (Var x)"
+| is_val_Const: "is_val (Const k)"
+| is_val_Unit: "is_val Unit"
+| is_val_Tuple: "is_val v1 \<Longrightarrow> is_val v2 \<Longrightarrow> is_val (Tup v1 v2)"
+| is_val_Lam: "is_exp e \<Longrightarrow> is_val (Lam x e)"
+
+equivariance is_exp
+nominal_inductive is_exp avoids is_exp_Def: x | is_val_Lam: x
+  by (auto simp add: fresh_star_def)
+
+
+inductive rule_Seq where
+  rule_Seq: "rule_Seq (Seq v e) e"
+equivariance rule_Seq
+
+
+
+inductive cc for R where
+  here: "R x y \<Longrightarrow> cc R x y"
+| under_Seql: "cc R x y \<Longrightarrow> cc R (Seq x e) (Seq y e)"
+| under_Seqr: "cc R x y \<Longrightarrow> cc R (Seq e x) (Seq e y)"
+| under_Barl: "cc R x y \<Longrightarrow> cc R (Bar x e) (Bar y e)"
+| under_Barr: "cc R x y \<Longrightarrow> cc R (Bar e x) (Bar e y)"
+| under_Appl: "cc R x y \<Longrightarrow> cc R (App x e) (App y e)"
+| under_Appr: "cc R x y \<Longrightarrow> cc R (App e x) (App e y)"
+| under_Def: "cc R x y \<Longrightarrow> cc R (Def z x) (Def z y)"
+| under_One: "cc R x y \<Longrightarrow> cc R (One x) (One y)"
+| under_All: "cc R x y \<Longrightarrow> cc R (All x) (All y)"
+| under_Tupl: "cc R x y \<Longrightarrow> cc R (Tup x e) (Tup y e)"
+| under_Tupr: "cc R x y \<Longrightarrow> cc R (Tup e x) (Tup e y)"
+| under_Lam: "cc R x y \<Longrightarrow> cc R (Lam z x) (Lam z y)"
+equivariance cc
+
+inductive_cases cc_SeqE[elim!, case_names]: "cc R (Seq e1 e2) e3"
+
+inductive_cases is_exp_SeqE[elim!]: "is_exp (Seq e1 e2)"
+inductive_cases is_val_SeqE[elim!]: "is_val (Seq e1 e2)"
+
+
+definition "VR = cc (rule_Seq)"
+
+lemma cc_local_confluence:
+  assumes "\<And> e1 e2 e3.
+   R e1 e2 \<Longrightarrow>
+   is_exp e1 \<Longrightarrow> is_exp e2 \<Longrightarrow> is_exp e3 \<Longrightarrow>
+   cc R e1 e3 \<Longrightarrow>
+  ((cc R)\<^sup>*\<^sup>* OO ((cc R)\<inverse>\<inverse>)\<^sup>*\<^sup>*) e2 e3"
+  shows "
+   is_exp e1 \<Longrightarrow> is_exp e2 \<Longrightarrow> is_exp e3 \<Longrightarrow>
+   cc R e1 e2 \<Longrightarrow> cc R e1 e3 \<Longrightarrow>
+  ((cc R)\<^sup>*\<^sup>* OO ((cc R)\<inverse>\<inverse>)\<^sup>*\<^sup>*) e2 e3"
+proof (induction e1 arbitrary: e2 e3 rule:exp.induct)
+  case (Seq x1 x2)
+
+  from `cc R (Seq x1 x2) e2`
+  show ?case
+  apply rule
+  proof(goal_cases)
+    case 1
+    then show ?case by (rule assms) (auto intro: Seq)
+  next
+    case (2 x1')
+    then show ?case sorry
+  next
+    case (3 y)
+    then show ?case sorry
+  qed
+    case goal1
+    apply rule
+      apply (erule assms;fact)
+     apply (rule Seq.IH(1))
+    using Seq apply fast
+    using Seq apply fast
+    using Seq apply fast
+
+         apply fact
+
+    using Seq
+    apply auto
+    apply (subst e2)
+    apply (rule Seq.IH)
+    
+next
+  case (Bar x1 x2)
+  then show ?case sorry
+next
+  case (App x1 x2)
+  then show ?case sorry
+next
+  case (Def x1 x2)
+  then show ?case sorry
+next
+  case (One x)
+  then show ?case sorry
+next
+  case (All x)
+  then show ?case sorry
+next
+  case (Var x)
+  then show ?case sorry
+next
+  case (Const x)
+  then show ?case sorry
+next
+  case Unit
+  then show ?case sorry
+next
+  case (Tup x1 x2)
+  then show ?case sorry
+next
+  case (Lam x1 x2)
+  then show ?case sorry
+qed
+  
+
+theorem local_confluence: 
+  assumes "is_exp e1" "is_exp e2" "is_exp e3"
+  assumes "R e1 e2" "R e1 e3"
+  shows "(R\<^sup>*\<^sup>* OO (R\<inverse>\<inverse>)\<^sup>*\<^sup>*) e2 e3"
+proof-
+  show ?thesis
+  using assms
+  proof (induction e1 rule:exp.induct)
+    case (Seq x1 x2)
+    from `R (Seq x1 x2) e2`
+    show ?case unfolding R_def
+    proof
+      
+      assume "rule_Seq (Seq x1 x2) e2"
+      thus ?case
+    
+    qed
+      
+  next
+    case (Bar x1 x2)
+    then show ?case sorry
+  next
+    case (App x1 x2)
+    then show ?case sorry
+  next
+    case (Def x1 x2)
+    then show ?case sorry
+  next
+    case (One x)
+    then show ?case sorry
+  next
+    case (All x)
+    then show ?case sorry
+  next
+    case (Var x)
+    then show ?case sorry
+  next
+    case (Const x)
+    then show ?case sorry
+  next
+    case Unit
+    then show ?case sorry
+  next
+    case (Tup x1 x2)
+    then show ?case sorry
+  next
+    case (Lam x1 x2)
+    then show ?case sorry
+  qed
+
 
 
 end
